GroupApproximation.lean
@@ -789,6 +789,7 @@ import GroupApproximation.Computability.RewriteSimulation
 import GroupApproximation.Monsters.NeumannContinuum
 import GroupApproximation.Computability.UnaryCounterSimulation
 import GroupApproximation.Computability.PostMachine
+import GroupApproximation.Computability.MachineRestrict
 import GroupApproximation.Computability.PostMachineHalting
 import GroupApproximation.Computability.HaltingReduction
 import GroupApproximation.Computability.RewriteSimulationOn
